src/GPUCSL/GPUCSL.v
@@ -8,20 +8,3 @@ Unset Strict Implicit.
 Require Import MyVector.
 Definition default ntrd : (Vector.t assn ntrd * Vector.t assn ntrd) := 
   (init (fun _ => Emp_assn), init (fun _ => Emp_assn)).
-
-Infix "+C" := (Ebinop (OP_arith OP_plus)) (at level 50, left associativity).
-Infix "*C" := (Ebinop (OP_arith OP_mult)) (at level 40, left associativity).
-Infix "-C" := (Ebinop (OP_arith OP_sub)) (at level 50, left associativity).
-Infix "<C" := (Ebinop (OP_comp OP_lt)) (at level 55).
-Infix "==C" := (Ebinop (OP_comp OP_eq)) (at level 55).
-Infix "/C" := (Ebinop (OP_arith OP_div)) (at level 40, left associativity).
-Infix "%C" := (Ebinop (OP_arith OP_mod)) (at level 40, left associativity).
-Infix "&&C" := (Ebinop (OP_bool OP_and)) (at level 56, left associativity).
-Infix "||C" := (Ebinop (OP_bool OP_or)) (at level 57, left associativity).
-Notation "'!C' x" := (Eunop OP_not x) (at level 39).
-Notation minC x y := (Ebinop (OP_arith OP_min) x y).
-Notation Zn := Z.of_nat.
-
-Coercion VZ : Z >-> val.
-Coercion VPtr : loc >-> val.
-Coercion Vval : val >-> lval.
